add char support and fix layout bug

rr_frontend/case_studies/tests/src/char.rs
@@ -1,0 +1,6 @@
+
+#[rr::params("c")]
+#[rr::args("c")]
+fn take_char(c: char) {
+
+}
