rr_frontend/case_studies/tests/src/enums.rs
@@ -1,11 +1,16 @@
-#![rr::import("refinedrust.extra_proofs.tests.enums", "typing")]
+#![rr::import("refinedrust.extra_proofs.tests.enums", "enums")]
 
+#[rr::refined_by("option (place_rfn {rt_of T})")]
 enum Option<T> {
+    #[rr::pattern("None")]
     None,
+    #[rr::pattern("Some" $ "x")]
+    #[rr::refinement("-[x]")]
     Some(T)
 }
 
 impl<T> Option<T> {
+    #[rr::returns("None")]
     pub fn none() -> Self {
         Self::None
     }
@@ -15,14 +20,30 @@ impl<T> Option<T> {
     }
 }
 
+
+#[rr::refined_by("result {rt_of T} {rt_of U}")]
+enum Result<T, U> {
+    #[rr::pattern("Ok" $ "x")]
+    #[rr::refinement("-[#x]")]
+    Ok(T),
+    #[rr::pattern("Err" $ "x")]
+    #[rr::refinement("-[#x]")]
+    Err(U),
+}
+
+impl<T, U> Result<T, U> {
+    #[rr::params("x")]
+    #[rr::args("x")]
+    pub fn foo(&self) {
+    }
+}
+
 #[repr(u8)]
 #[rr::refined_by("sizes")]
 enum sizes {
     #[rr::pattern("Sz1")]
-    #[rr::variant("()")]
     Sz1 = 2,
     #[rr::pattern("Sz2")]
-    #[rr::variant("()")]
     Sz2,
 }
 
