theories/caesium/char.v
@@ -1,0 +1,31 @@
+From stdpp Require Export strings.
+From stdpp Require Import gmap list.
+From caesium Require Export base layout int_type.
+Set Default Proof Using "Type".
+
+Definition char_it : int_type := u32.
+Definition char_layout : layout := it_layout char_it.
+
+(* From https://doc.rust-lang.org/std/primitive.char.html:
+"A char is a ‘Unicode scalar value’, which is any ‘Unicode code point’ other than a surrogate code point. This has a fixed numerical definition: code points are in the range 0 to 0x10FFFF, inclusive. Surrogate code points, used by UTF-16, are in the range 0xD800 to 0xDFFF."
+ *)
+Definition is_valid_char (z : Z) :=
+  (0 ≤ z ≤ 1114111)%Z ∧ ¬ (55296 ≤ z ≤ 57343)%Z.
+
+Global Instance is_valid_char_dec z : Decision (is_valid_char z).
+Proof. solve_decision. Defined.
+
+Lemma is_valid_char_in_char_it z :
+  is_valid_char z → z ∈ char_it.
+Proof.
+  rewrite /is_valid_char.
+  rewrite /elem_of /int_elem_of_it.
+  rewrite /char_it.
+  rewrite /min_int/max_int/=/int_modulus.
+  rewrite /bits_per_int/bytes_per_int/byte.bits_per_byte.
+  simpl.
+  nia.
+Qed.
+
+Lemma char_layout_wf : layout_wf char_layout.
+Proof. apply int_type_layout_wf. Qed.
